Great question â€” this is **the heart of linear regression**.
Iâ€™ll derive **âˆ‚MSE / âˆ‚m** **slowly, step by step**, with **zero jumps**.

We start from scratch ğŸ‘‡

---

# ğŸ¯ Goal

Find the **derivative of MSE with respect to `m`**

---

## 1ï¸âƒ£ Mean Squared Error (MSE)

[
\text{MSE} = \frac{1}{n}\sum_{i=1}^{n} (y_i - \hat{y}_i)^2
]

---

## 2ï¸âƒ£ Predicted Value (Å·)

For linear regression:

[
\hat{y}_i = m x_i + c
]

Substitute this into MSE:

[
\text{MSE} = \frac{1}{n}\sum_{i=1}^{n} (y_i - (m x_i + c))^2
]

---

## 3ï¸âƒ£ Rewrite the Expression (important)

[
\text{MSE} = \frac{1}{n}\sum_{i=1}^{n} (y_i - m x_i - c)^2
]

We will now **differentiate this with respect to `m`**.

---

## 4ï¸âƒ£ Take Derivative w.r.t. `m`

[
\frac{\partial}{\partial m}\left[\frac{1}{n}\sum (y_i - m x_i - c)^2\right]
]

### Step 1: Take constant out

[
= \frac{1}{n}\sum \frac{\partial}{\partial m}(y_i - m x_i - c)^2
]

---

## 5ï¸âƒ£ Apply Chain Rule

Let:
[
u = (y_i - m x_i - c)
]

Then:
[
\frac{d}{dm}(u^2) = 2u \cdot \frac{du}{dm}
]

---

## 6ï¸âƒ£ Compute Inner Derivative

[
\frac{d}{dm}(y_i - m x_i - c) = -x_i
]

(because `yáµ¢` and `c` are constants)

---

## 7ï¸âƒ£ Combine Everything

[
\frac{\partial}{\partial m}(y_i - m x_i - c)^2
= 2(y_i - m x_i - c)(-x_i)
]

---

## 8ï¸âƒ£ Final Expression

[
\frac{\partial \text{MSE}}{\partial m}
= \frac{1}{n}\sum 2(y_i - m x_i - c)(-x_i)
]

Simplify:

[
= -\frac{2}{n}\sum x_i (y_i - \hat{y}_i)
]

---

## âœ… FINAL ANSWER

[
\boxed{
\frac{\partial \text{MSE}}{\partial m}
= -\frac{2}{n}\sum_{i=1}^{n} x_i (y_i - \hat{y}_i)
}
]

---

## ğŸ” Gradient Descent Update Rule

[
m_{\text{new}} = m_{\text{old}} - \eta \frac{\partial \text{MSE}}{\partial m}
]

Substitute:

[
m = m + \frac{2\eta}{n}\sum x_i (y_i - \hat{y}_i)
]

---

## ğŸ§  Intuition (Very Important)

* If prediction is **too small**, `(y - Å·)` is positive â†’ slope increases
* If prediction is **too large**, `(y - Å·)` is negative â†’ slope decreases
* Gradient descent **nudges the line** in the correct direction

---

## ğŸ¯ What You Should Remember for Exams / Interviews

âœ” MSE formula
âœ” Substitute Å· = mx + c
âœ” Use chain rule
âœ” Final gradient formula
âœ” Plug into gradient descent

------Perfect â€” this one is **simpler than âˆ‚/âˆ‚m**, and Iâ€™ll derive it **cleanly, step by step**, no skips.

---

# ğŸ¯ Goal

Find the **derivative of MSE with respect to `c`**

---

## 1ï¸âƒ£ Mean Squared Error (MSE)

[
\text{MSE} = \frac{1}{n}\sum_{i=1}^{n} (y_i - \hat{y}_i)^2
]

---

## 2ï¸âƒ£ Predicted Value (Å·)

For linear regression:

[
\hat{y}_i = m x_i + c
]

Substitute into MSE:

[
\text{MSE} = \frac{1}{n}\sum_{i=1}^{n} (y_i - m x_i - c)^2
]

---

## 3ï¸âƒ£ Differentiate w.r.t. `c`

[
\frac{\partial}{\partial c}
\left[
\frac{1}{n}\sum (y_i - m x_i - c)^2
\right]
]

Take constant out:

[
= \frac{1}{n}\sum
\frac{\partial}{\partial c}(y_i - m x_i - c)^2
]

---

## 4ï¸âƒ£ Apply Chain Rule

Let:
[
u = (y_i - m x_i - c)
]

[
\frac{d}{dc}(u^2) = 2u \cdot \frac{du}{dc}
]

---

## 5ï¸âƒ£ Inner Derivative

[
\frac{d}{dc}(y_i - m x_i - c) = -1
]

---

## 6ï¸âƒ£ Combine

[
\frac{\partial}{\partial c}(y_i - m x_i - c)^2
= 2(y_i - m x_i - c)(-1)
]

---

## 7ï¸âƒ£ Final Expression

[
\frac{\partial \text{MSE}}{\partial c}
= \frac{1}{n}\sum 2(y_i - m x_i - c)(-1)
]

Simplify:

[
\boxed{
\frac{\partial \text{MSE}}{\partial c}
= -\frac{2}{n}\sum_{i=1}^{n} (y_i - \hat{y}_i)
}
]

---

## ğŸ” Gradient Descent Update Rule for `c`

[
c_{\text{new}} = c_{\text{old}} - \eta \frac{\partial \text{MSE}}{\partial c}
]

Substitute:

[
\boxed{
c = c + \frac{2\eta}{n}\sum (y_i - \hat{y}_i)
}
]

---

## ğŸ§  Intuition (IMPORTANT)

* If predictions are **consistently too low**, sum of errors is positive â†’ increase `c`
* If predictions are **too high**, sum of errors is negative â†’ decrease `c`
* `c` shifts the line **up or down**

---

## ğŸ§¾ Final Gradient Formulas (MEMORIZE)

[
\frac{\partial \text{MSE}}{\partial m}
= -\frac{2}{n}\sum x_i (y_i - \hat{y}_i)
]

[
\frac{\partial \text{MSE}}{\partial c}
= -\frac{2}{n}\sum (y_i - \hat{y}_i)
]

---

If you want next, I can:

* Do **manual numeric calculation**
* Show **one gradient descent iteration**
* Explain **why squared error works**
* Connect this to **vector/matrix form**

Just say ğŸ‘

